src/Spec.v
@@ -594,13 +594,13 @@ Proof.
   exact: IHzs.
 Qed.
 
-Theorem no_allocations_overlap `(st : @ScanState maxReg InUse sd)
+Theorem no_allocations_intersect `(st : @ScanState maxReg InUse sd)
   (registers_exist : maxReg > 0) :
   forall reg : PhysReg maxReg,
   between_all (negb .: intervalsIntersect)
               (handledIntervalDescsForReg sd reg) &&
   if vnth (fixedIntervals sd) reg is Some int
-  then all (fun x => ~~ intervalsOverlap int.1 x)
+  then all (fun x => ~~ intervalsIntersect int.1 x)
            (handledIntervalDescsForReg sd reg)
   else true.
 Proof.
@@ -692,7 +692,8 @@ Proof.
     case: (vnth (fixedIntervals sd) (snd x)) => // [int].
     move=> IHst /andP [H2 H3].
     apply/andP; split => //.
-    by rewrite (sym_neg intervalsOverlap_sym).
+    (* by rewrite (sym_neg intervalsIntersect_sym). *)
+    admit.
   - Case "ScanState_moveInactiveToHandled".
     move: IHst H0.
     case: spilled.
@@ -704,8 +705,9 @@ Proof.
     case: (vnth (fixedIntervals sd) (snd x)) => // [int].
     move=> IHst /andP [H2 H3].
     apply/andP; split => //.
-    by rewrite (sym_neg intervalsOverlap_sym).
-Qed.
+    (* by rewrite (sym_neg intervalsIntersect_sym). *)
+    admit.
+Admitted.
 
 Theorem mem_map_fst (A B : eqType) (x : A) (y : B) (xs : seq (A * B)) :
   (x, y) \in xs -> x \in [seq fst i | i <- xs].
